\begin{latin}
    \section*{\lr{Exercises}}
    (19.1) (a):\
    \begin{alignat*}{2}
        for \to He \Longrightarrow E &= \frac{1}{2} m(v_x ^2 + v_y ^2 + v_z ^2)\\
        n = 3 \Longrightarrow \left \langle E \right \rangle &= \frac{n}{2}k_B T = \frac{3}{2}k_B T\\
        for \to Xe \Longrightarrow E &= \frac{1}{2} m(v_x ^2 + v_y ^2 + v_z ^2)\\
        n = 3 \Longrightarrow \left \langle E \right \rangle &= \frac{n}{2}k_B T = \frac{3}{2}k_B T\\
        for \to Ar \Longrightarrow E &= \frac{1}{2} m(v_x ^2 + v_y ^2 + v_z ^2)\\
        n = 3 \Longrightarrow \left \langle E \right \rangle &= \frac{n}{2}k_B T = \frac{3}{2}k_B T\\
        for \to Kr \Longrightarrow E &= \frac{1}{2} m(v_x ^2 + v_y ^2 + v_z ^2)\\
        n = 3 \Longrightarrow \left \langle E \right \rangle &= \frac{n}{2}k_B T = \frac{3}{2}k_B T
    \end{alignat*}
    we have to do four separate calculations.\\
    \begin{latin}
        (19.3):
        \begin{alignat*}{2}
            v_{(r)} &= \frac{A}{r^n} - \frac{B}{r}\\
            (a) \to (\frac{dV}{dr})_{r_0} &=0\\
            (b) \to V_{(x)}&= V_{(x_0)} + (\frac{\partial V}{\partial x})_{x_0} (x-x_0) + \frac{1}{2}(\frac{\partial V^2}{\partial^2 x})_{x_0} (x-x_0)^2 + \dots \\
            (a) and (b) \Longrightarrow V_{(x)}&= V_{(x_0)} + \frac{1}{2}(\frac{\partial V^2}{\partial^2 x})_{x_0} (x-x_0)^2  +\dots\\
            v_{(r)} &= \frac{A}{r^n} - \frac{B}{r}\\
            (a)\to \frac{d}{dr}(v_{(r)} = \frac{A}{r^n} - \frac{B}{r}) &= 0\\
            -\frac{nA}{r_0 ^n+1}+ \frac{B}{r_0 ^2} &=0\\
            r_0 ^n-1 &=\frac{nA}{B} \\
            \Longrightarrow V = V_{(x_0)} + \frac{1}{2}(\frac{\partial V^2}{\partial^2 x})_{x_0} (x-x_0)^2  &= V_0 + \alpha (r-r_0)^2\\
            f = 2 \Longrightarrow  \left \langle E \right \rangle &= \frac{f}{2} k_B T =k_B T\\
            \Longrightarrow \left \langle E \right \rangle &=k_B T\\
        \end{alignat*}
        (19.4):
        \begin{alignat*}{2}
            \left \langle E \right \rangle &= \sum_{n=1}^n \alpha_i \left \langle x_i ^2 \right \rangle\\
            \Longrightarrow\left \langle x_i ^2 \right \rangle &= \frac{\left \langle E \right \rangle}{\alpha_i}\\
            \left \langle E \right \rangle &= \frac{1}{2} k_B T\\
            \Longrightarrow \left \langle x_i ^2 \right \rangle &= \frac{k_B T}{2\alpha_i}\\
        \end{alignat*}
        (19.5):
        \begin{alignat*}{2}
            E &= \alpha |x|\\
            \left \langle E \right \rangle &= \int_{-\infty}^{\infty} E P_{(x)}dx \\
            &= \frac{\int_{-\infty}^{\infty} \alpha x e^{-\beta\alpha x^2}dx}{\int_{-\infty}^{\infty}  e^{-\beta\alpha x^2}dx}\\
            &= \frac{1}{\beta}\\
            &= k_B T \\       
        \end{alignat*}
        (19.6):
        \begin{alignat*}{2}
            E &= \alpha |x|^n\\
            \left \langle E \right \rangle &= \int_{-\infty}^{\infty} E P_{(x)}dx \\
            &= \frac{\int_{-\infty}^{\infty} \alpha |x|^n e^{-\beta\alpha x^2}dx}{\int_{-\infty}^{\infty}  e^{-\beta\alpha x^2}dx}\\
            &= \frac{1}{n\beta}\\
            \xi = \frac{1}{n} \Longrightarrow \left \langle E \right \rangle&=\xi k_B T \\ 
        \end{alignat*}

    \end{latin}
\end{latin}


