\begin{latin}   
   \section*{Exercises}
    (16.1) (a):\


    \begin{alignat*}{3}
        \textmd{ First low }&:dU &&= TdS - pdv\\
        \textmd{ Enthalpy }&:H &&= U + pv\\
        \textmd{ Helmholtz function }&:F &&= U - TS\\
        \textmd{ Gibbd function }&:G &&= U + pv - TS
    \end{alignat*}
    give $dU , dH, dF, dG$ in terms of $T, S, p, V$

    \begin{alignat*}{2}
        dU &= TdS - pdv\\\\
        dH &= dU + pdV + Vdp\\
        &= Tds - pdV  + pdV + Vdp\\
        &= Tds + Vdp\\\\
        dF &= dU - TdS - SdT\\
        &=TdS - pdV -TdS - SdT\\
        &= -pdV - SdT\\\\
        dG &= dH - TdS - SdT\\
        &= TdS - Vdp -TdS - SdT \\
        &= -SdT + pdV\\ 
    \end{alignat*}
    (16.3): \\
    \begin{alignat*}{2}
    dU &= TdS - pdv\\
    dS &= (\frac{\partial S}{\partial T})_v dT + (\frac{\partial S}{\partial V})_T dV\\
    \Longrightarrow dU &= T[\frac{\partial S}{\partial T})_v dT + (\frac{\partial S}{\partial V})_T dV] +pdV\\
    &=T(\frac{\partial S}{\partial T})_v dT+ [T(\frac{\partial S}{\partial V})_T dV -p]dV\\\\
    (\frac{\partial U}{\partial V})_T \Rightarrow
    \begin{cases} 
    \beta_p = \frac{1}{V}(\frac{\partial V}{\partial T})_p ) \\
    \kappa_T = - \frac{1}{V}(\frac{\partial V}{\partial p})_T )
    \end{cases}
    \Longrightarrow\frac{\beta_p}{\kappa_T} &= (\frac{\partial p}{\partial T})_V )\\\\
    1)\to(\frac{\partial S}{\partial T})_v &= [T(\frac{\partial S}{\partial V})_T -p]\\
    2)\to (\frac{\partial S}{\partial V})_T &= (\frac{\partial p}{\partial T})_V\\
    1and2\Longrightarrow (\frac{\partial U}{\partial V})_T  &= [T(\frac{\partial p}{\partial T})_V -p ]\\
    \Longrightarrow dV &= (\frac{\partial V}{\partial T})_pdT + (\frac{\partial V}{\partial p})_T)dp \\ 
    in isochoric \Longrightarrow (\frac{\partial V}{\partial p})_T dp &= -(\frac{\partial V}{\partial T})_pdT\\
    \Longrightarrow dp &= - \frac{(\frac{\partial V}{\partial T})_p}{(\frac{\partial V}{\partial p})_T}dT\\
    (\frac{\partial p}{\partial T})_V &= - \frac{(\frac{\partial V}{\partial T})_p}{(\frac{\partial V}{\partial p})_T}dT\\
    and (\frac{\partial p}{\partial T})_V &= \frac{\beta_p}{\kappa_T}\\
    \Longrightarrow (\frac{\partial U}{\partial V})_T &= [T(\frac{\beta_p}{\kappa_T}) - p]\\
    in.the.other \to C_p -C_V &= \frac{VT\beta_p }{\kappa_T}\\
    \Longrightarrow \frac{C_p - C_V}{V\beta_p} &= \frac{T\beta_p}{\kappa_T}\\
    \Longrightarrow (\frac{\partial U}{\partial V})_T &= [\frac{C_p - C_V}{V\beta_p} -p]
    \end{alignat*}

    (16.4) (a): \
    \begin{alignat*}{3}
        U_(S,V) &= TdS - pdV\\
    \begin{cases} 
        dS = (\frac{\partial S}{\partial T})_v dT +(\frac{\partial S}{\partial V})_T dV\\
        (\frac{\partial S}{\partial T})_v = \frac{C_V}{T}\\
        dV = -V(\frac{dp}{p})
    \end{cases}
        \Longrightarrow&= T(\frac{\partial S}{\partial T})_v dT + T(\frac{\partial S}{\partial V})_T (-Vdp) + Vdp= U_(T,p)\\\\
    \end{alignat*}

    (b):\
    \begin{alignat*}{2}
        Due\ to\ the\ 3Exercise \Longrightarrow (\frac{\partial U}{\partial V})_T &= [T((\frac{\partial S}{\partial V})_T - p]\\
        \frac{p}{T} &= (\frac{\partial S}{\partial V})_T - (\frac{\partial U}{\partial V})_T \frac{1}{T}\\
        \begin{cases} 
            (\frac{\partial S}{\partial V})_T = f_(V)\\
            (\frac{\partial U}{\partial V})_T \frac{1}{T} = \int(\frac{\partial U}{\partial V})_T \frac{dT}{T^2}
        \end{cases}\\
        \Longrightarrow \frac{p}{T} &= \int(\frac{\partial U}{\partial V})_T \frac{dT}{T^2} + f_(V)
    \end{alignat*}\\\\

    (16.5):\
    \begin{alignat*}{2}
        dU &= TdS - pdv\\
        dS &= (\frac{\partial S}{\partial T})_v dT + (\frac{\partial S}{\partial V})_T dV\\
        \Longrightarrow dU &= T[\frac{\partial S}{\partial T})_v dT + (\frac{\partial S}{\partial V})_T dV] +dV\\
        &=T(\frac{\partial S}{\partial T})_v dT+ [T(\frac{\partial S}{\partial V})_T dV -p]dV\\
        isothermal\Longrightarrow dU&= [T(\frac{\partial S}{\partial V})_T dV -p]dV\\
        \Longrightarrow (\frac{\partial U}{\partial V})_T &= [T((\frac{\partial S}{\partial V})_T - p]\\
        Example\ 16.5\ \to (\frac{\partial S}{\partial V})_T = (\frac{\partial p}{\partial T})_V\Longrightarrow p &= T(\frac{\partial p}{\partial T})_V - (\frac{\partial U}{\partial V})_T \\
    \end{alignat*}\\

    (16.6):\
    \begin{alignat*}{2}
        dS &= (\frac{\partial S}{\partial T})_v dT + (\frac{\partial S}{\partial V})_T dV\\
        \begin{cases}
            \frac{\partial S}{\partial T})_v dT =\frac{C_V}{T} dT\\
            (\frac{\partial S}{\partial V})_T = (\frac{\partial p}{\partial T})_V
        \end{cases}\\\\
        \Longrightarrow dS&= \frac{C_V}{T} dT + (\frac{\partial p}{\partial T})_V dV \to
        \begin{cases}
            dV = -V \frac{dp}{p}\\
            (\frac{\partial p}{\partial T})_V = \frac{R}{V}
        \end{cases}\\\\
        \Longrightarrow S &= C_p ln\ T - Rln\ p + costant
    \end{alignat*}

\end{latin}
